theories/rule_misc.v
@@ -799,7 +799,7 @@ From HypVeri Require Import RAs.
     inversion H2;subst x1.
     clear H2.
     rewrite H0 H1.
-    do 8 f_equal.
+    do 6 f_equal.
     rewrite /get_vm_page_table /get_page_tables /=.
     destruct (decide (get_current_vm σ = x0)).
     subst x0.
@@ -828,13 +828,13 @@ From HypVeri Require Import RAs.
 
 
   Lemma get_pagetable_gmap_checkb {Perm:Type} {σ i s} proj (checkb: Perm -> bool) p:
-   (get_pagetable_gmap σ proj checkb) !! i = Some (DfracOwn 1, to_agree (GSet s))->
+   (get_pagetable_gmap σ proj checkb) !! i = Some (GSet s)->
    (p ∈ s <->
     ∃ perm, (proj (get_vm_page_table σ i)) !! p =Some perm ∧ checkb perm = true).
   Proof.
     intros.
     rewrite /get_access_gmap in H.
-    apply (elem_of_list_to_map_2 _ i (DfracOwn 1, to_agree (GSet s))) in H.
+    apply (elem_of_list_to_map_2 _ i (GSet s)) in H.
     inv_map_in. clear H0.
     inversion H.
     subst.
@@ -863,7 +863,7 @@ From HypVeri Require Import RAs.
   Qed.
 
   Lemma get_owned_gmap_is_owned {σ i sown} p:
-   (get_owned_gmap σ) !! i = Some (DfracOwn 1, to_agree (GSet sown))->
+   (get_owned_gmap σ) !! i = Some (GSet sown)->
    (p ∈ sown <->
     ∃ perm, (get_vm_page_table σ i).1 !! p =Some perm ∧ is_owned perm = true).
   Proof.
@@ -873,7 +873,7 @@ From HypVeri Require Import RAs.
   Qed.
 
   Lemma get_access_gmap_is_accessible {σ i sacc} p:
-   (get_access_gmap σ) !! i = Some (DfracOwn 1, to_agree (GSet sacc))->
+   (get_access_gmap σ) !! i = Some (GSet sacc)->
    (p ∈ sacc <->
     ∃ perm, (get_vm_page_table σ i).2 !! p =Some perm ∧ is_accessible perm = true).
   Proof.
@@ -883,7 +883,7 @@ From HypVeri Require Import RAs.
   Qed.
 
   Lemma get_excl_gmap_is_exclusive_true {σ i sexcl} p:
-   (get_excl_gmap σ) !! i = Some (DfracOwn 1, to_agree (GSet sexcl))->
+   (get_excl_gmap σ) !! i = Some (GSet sexcl)->
    (p ∈ sexcl<->
     ∃ perm, (get_vm_page_table σ i).2 !! p =Some perm ∧ is_exclusive perm = true).
   Proof.
@@ -897,9 +897,9 @@ From HypVeri Require Import RAs.
    sps = (list_to_set ps)->
    i = (get_current_vm σ) ->
    checkb NoAccess = false ->
-   (get_pagetable_gmap σ (λ pt,pt.2) checkb) !! i = Some (DfracOwn 1, to_agree (GSet s)) ->
+   (get_pagetable_gmap σ (λ pt,pt.2) checkb) !! i = Some (GSet s) ->
    (get_pagetable_gmap (update_access_batch σ ps NoAccess)  (λ pt,pt.2) checkb) =
-   <[(get_current_vm σ):= (DfracOwn 1, to_agree (GSet (s ∖ sps ) ))]>(get_pagetable_gmap σ (λ pt,pt.2) checkb).
+   <[(get_current_vm σ):= (GSet (s ∖ sps))]>(get_pagetable_gmap σ (λ pt,pt.2) checkb).
   Proof.
     intros Hsps Hi Hcheckb Hlookup.
     rewrite /get_pagetable_gmap.
@@ -988,13 +988,12 @@ From HypVeri Require Import RAs.
         apply Hgoal.
     - rewrite (lookup_insert_ne _ i i0 _);eauto.
       set (l:= (map (λ v : VMID,
-                           (v, (DfracOwn 1,
-                                to_agree (GSet (list_to_set
-                                                  (map (λ p : PID * access, p.1)
-                                                       (map_to_list (filter (λ p : PID * access, checkb p.2 = true)
-                                                                            (get_vm_page_table σ v).2)))))))) list_of_vmids)) in *.
+                      (v, (GSet (list_to_set
+                            (map (λ p : PID * access, p.1)
+                                  (map_to_list (filter (λ p : PID * access, checkb p.2 = true)
+                                        (get_vm_page_table σ v).2))))))) list_of_vmids)) in *.
       destruct (list_to_map l !! i0) eqn:Heqn.
-      + apply (elem_of_list_to_map_2 l i0 c) in Heqn.
+      + apply (elem_of_list_to_map_2 l i0 g) in Heqn.
         apply elem_of_list_In in Heqn.
         apply in_map_iff in Heqn.
         inversion Heqn;clear Heqn.
@@ -1003,12 +1002,12 @@ From HypVeri Require Import RAs.
         *  intros.
            inv_map_in.
            inversion H.
-           do 7 f_equal.
+           do 5 f_equal.
            rewrite /get_vm_page_table update_access_batch_preserve_other_page_tables //.
         * inv_map_in.
           exists i0.
           split;eauto.
-          do 8 f_equal.
+          do 6 f_equal.
           rewrite /get_vm_page_table update_access_batch_preserve_other_page_tables //.
       + apply (@not_elem_of_list_to_map_2 VMID (gmap VMID) _ _ _ _ _ _ _ _ gmap_finmap) in Heqn.
         apply (@not_elem_of_list_to_map_1 VMID (gmap VMID) _ _ _ _ _ _ _ _ gmap_finmap).
@@ -1029,30 +1028,30 @@ From HypVeri Require Import RAs.
         destruct H0.
         split;eauto.
         rewrite -H0.
-        do 8 f_equal.
+        do 6 f_equal.
         rewrite /get_vm_page_table update_access_batch_preserve_other_page_tables //.
         destruct x.
         inversion H0.
         by subst.
   Qed.
 
-  Lemma update_access_batch_update_access_diff{ σ i sacc} {sps:gset PID} (ps: list PID):
+  Lemma update_access_batch_update_access_diff{σ i sacc} {sps:gset PID} (ps: list PID):
     sps = (list_to_set ps)->
     i = (get_current_vm σ) ->
-    (get_access_gmap σ) !! i = Some (DfracOwn 1, to_agree (GSet sacc)) ->
+    (get_access_gmap σ) !! i = Some  (GSet sacc) ->
     get_access_gmap (update_access_batch σ ps NoAccess) =
-    <[(get_current_vm σ):= (DfracOwn 1, to_agree (GSet (sacc∖ sps ) ))]>(get_access_gmap σ).
+    <[(get_current_vm σ):= (GSet (sacc∖ sps))]>(get_access_gmap σ).
   Proof.
     intros.
     apply (@update_access_batch_update_pagetable_diff _ i);eauto.
   Qed.
 
-  Lemma update_access_batch_update_excl_diff{ σ i sexcl} {sps:gset PID} (ps: list PID):
+  Lemma update_access_batch_update_excl_diff{σ i sexcl} {sps:gset PID} (ps: list PID):
     sps = (list_to_set ps)->
     i = (get_current_vm σ) ->
-    (get_excl_gmap σ) !! i = Some (DfracOwn 1, to_agree (GSet sexcl)) ->
+    (get_excl_gmap σ) !! i = Some (GSet sexcl) ->
     get_excl_gmap (update_access_batch σ ps NoAccess) =
-    <[(get_current_vm σ):= (DfracOwn 1, to_agree (GSet (sexcl ∖ sps ) ))]>(get_excl_gmap σ).
+    <[(get_current_vm σ):= (GSet (sexcl ∖ sps))]>(get_excl_gmap σ).
   Proof.
     intros.
     apply (@update_access_batch_update_pagetable_diff _ i);eauto.
@@ -1061,164 +1060,163 @@ From HypVeri Require Import RAs.
   Lemma update_ownership_batch_update_pagetable_union{σ i sown} {sps:gset PID} (ps: list PID):
    sps = (list_to_set ps)->
    i = (get_current_vm σ)->
-   (get_owned_gmap σ) !! i = Some (DfracOwn 1, to_agree (GSet sown)) ->
+   (get_owned_gmap σ) !! i = Some (GSet sown) ->
    get_owned_gmap (update_ownership_batch σ ps Owned) =
-   <[i:= (DfracOwn 1, to_agree (GSet (sown ∪ sps ) ))]>(get_owned_gmap σ).
+   <[i:= (GSet (sown ∪ sps))]>(get_owned_gmap σ).
   Proof.
-      intros.
-      rewrite /get_owned_gmap /get_pagetable_gmap.
-      apply (@map_eq VMID (gmap VMID) _ _ _ _ _ _ _ _ gmap_finmap);eauto.
-      intro.
-      destruct(decide (i0 = i)).
-      - subst i0. rewrite lookup_insert.
-        assert(Hgoal: list_to_set
+    intros.
+    rewrite /get_owned_gmap /get_pagetable_gmap.
+    apply (@map_eq VMID (gmap VMID) _ _ _ _ _ _ _ _ gmap_finmap);eauto.
+    intro.
+    destruct(decide (i0 = i)).
+    - subst i0. rewrite lookup_insert.
+      assert(Hgoal: list_to_set
                        (map (λ p : PID * ownership, p.1)
                             (map_to_list (filter (λ p : PID * ownership, is_owned p.2 = true)
                           (get_vm_page_table (update_ownership_batch σ ps Owned) i).1))) = sown ∪ sps).
-        {
-          apply set_eq.
-          intro.
-          rewrite  elem_of_list_to_set.
-          split.
-          * intros.
-            inv_map_in.
-            apply elem_of_list_In in H3.
-            apply (elem_of_map_to_list' _ x0) in H3.
-            apply map_filter_lookup_Some in H3.
-            destruct H3.
-            simplify_eq /=.
-            rewrite /get_vm_page_table /get_page_tables /update_ownership_batch
-                    /update_ownership_global_batch //= in H3.
-            rewrite vlookup_insert in H3.
-            apply elem_of_union.
-            induction ps; simpl in *.
-            -- left.
-               apply (get_owned_gmap_is_owned x0.1 H1).
-               exists (x0.2).
-               split;eauto.
-            -- destruct (decide (a=x0.1)).
-               right;set_solver.
-               assert (Himp :(x0.1 ∈ sown ∨ x0.1 ∈ ((list_to_set ps):gset PID))
-                             ->(x0.1 ∈ sown ∨ x0.1 ∈ {[a]} ∪ ((list_to_set ps):gset PID))).
-               { intros. destruct H. left;done. right; set_solver. }
-               apply Himp.
-               apply IHps;eauto.
-               rewrite lookup_insert_ne in H3;done.
-          * intros.
-            apply elem_of_union in H2.
-            destruct H2.
-            apply (get_owned_gmap_is_owned x H1) in H2;eauto.
-            destruct H2.
-            destruct H2.
-            inv_map_in.
-            exists (x,x0).
-            split;eauto.
-            apply elem_of_list_In .
-            apply elem_of_map_to_list.
-            apply map_filter_lookup_Some.
-            rewrite /get_vm_page_table /get_page_tables /update_ownership_batch
-                    /update_ownership_global_batch /=.
-            rewrite -H0 vlookup_insert.
-            destruct H1;split;eauto.
-            generalize dependent sps.
-            induction ps;simpl in *.
-            done.
-            intros.
-            destruct (decide (x=a)).
-            subst a.
-            rewrite lookup_insert.
-            rewrite /is_owned in H3.
-            destruct x0;eauto.
-            done.
-            rewrite lookup_insert_ne;eauto.
-            inv_map_in.
-            exists (x,Owned).
-            split;eauto.
-            apply elem_of_list_In .
-            apply elem_of_map_to_list.
-            apply map_filter_lookup_Some.
-            rewrite /get_vm_page_table /get_page_tables /update_ownership_batch
-                    /update_ownership_global_batch /=.
-            split;eauto.
-            rewrite -H0 vlookup_insert //=.
-            generalize dependent sps.
-            induction ps;simpl in *.
-            intros.
-            set_solver.
-            intros.
-            destruct (decide (x=a)).
-            subst a.
-            rewrite lookup_insert //.
-            rewrite lookup_insert_ne;eauto.
-            apply (IHps (list_to_set ps));eauto.
-            set_solver.
-        }
-        apply (@elem_of_list_to_map_1' VMID (gmap VMID) _ _ _ _ _ _ _ _ gmap_finmap).
-        + intros.
+      {
+        apply set_eq.
+        intro.
+        rewrite  elem_of_list_to_set.
+        split.
+        * intros.
           inv_map_in.
-          inversion H2.
-          do 3 f_equal.
-          clear H6 H3 H2.
-          subst x.
-          symmetry.
-          apply Hgoal.
-        + inv_map_in.
-          exists i.
-          split;[|apply in_list_of_vmids].
-          do 4 f_equal.
-          apply Hgoal.
-      - rewrite (lookup_insert_ne _ i i0 _);eauto.
-        set (l:= (map
-                    (λ v : VMID,
-                           (v, (DfracOwn 1,
-                                to_agree (GSet
-                                            (list_to_set
-                                               (map (λ p : PID * ownership, p.1)
-                                                    (map_to_list
-                                                       (filter (λ p : PID * ownership, is_owned p.2 = true) (get_vm_page_table σ v).1))))))))
-                    list_of_vmids)) in *.
-        destruct (list_to_map l !! i0) eqn:Heqn.
-        + apply (elem_of_list_to_map_2 l i0 c) in Heqn.
-          apply elem_of_list_In in Heqn.
-          apply in_map_iff in Heqn.
-          inversion Heqn;clear Heqn.
-          destruct H2 as [H3 HIn];inversion H3;subst;clear H3.
-          apply (@elem_of_list_to_map_1' VMID (gmap VMID) _ _ _ _ _ _ _ _ gmap_finmap).
-          *  intros.
-             inv_map_in.
-             inversion H.
-             do 7 f_equal.
-             rewrite /get_vm_page_table update_ownership_batch_preserve_other_page_tables //.
-          * inv_map_in.
-            exists i0.
-            split;eauto.
-            do 8 f_equal.
-            rewrite /get_vm_page_table update_ownership_batch_preserve_other_page_tables //.
-        + apply (@not_elem_of_list_to_map_2 VMID (gmap VMID) _ _ _ _ _ _ _ _ gmap_finmap) in Heqn.
-          apply (@not_elem_of_list_to_map_1 VMID (gmap VMID) _ _ _ _ _ _ _ _ gmap_finmap).
-          intro P.
-          apply Heqn.
-          apply elem_of_list_In.
-          apply in_map_iff.
-          apply elem_of_list_In in P.
-          apply in_map_iff in P.
-          destruct P.
-          exists x.
+          apply elem_of_list_In in H3.
+          apply (elem_of_map_to_list' _ x0) in H3.
+          apply map_filter_lookup_Some in H3.
+          destruct H3.
+          simplify_eq /=.
+          rewrite /get_vm_page_table /get_page_tables /update_ownership_batch
+                  /update_ownership_global_batch //= in H3.
+          rewrite vlookup_insert in H3.
+          apply elem_of_union.
+          induction ps; simpl in *.
+          -- left.
+             apply (get_owned_gmap_is_owned x0.1 H1).
+             exists (x0.2).
+             split;eauto.
+          -- destruct (decide (a=x0.1)).
+             right;set_solver.
+             assert (Himp :(x0.1 ∈ sown ∨ x0.1 ∈ ((list_to_set ps):gset PID))
+                           ->(x0.1 ∈ sown ∨ x0.1 ∈ {[a]} ∪ ((list_to_set ps):gset PID))).
+             { intros. destruct H. left;done. right; set_solver. }
+             apply Himp.
+             apply IHps;eauto.
+             rewrite lookup_insert_ne in H3;done.
+        * intros.
+          apply elem_of_union in H2.
           destruct H2.
+          apply (get_owned_gmap_is_owned x H1) in H2;eauto.
+          destruct H2.
+          destruct H2.
+          inv_map_in.
+          exists (x,x0).
           split;eauto.
-          apply in_map_iff.
-          apply in_map_iff in H3.
-          destruct H3.
-          exists x0.
-          destruct H3.
+          apply elem_of_list_In .
+          apply elem_of_map_to_list.
+          apply map_filter_lookup_Some.
+          rewrite /get_vm_page_table /get_page_tables /update_ownership_batch
+                  /update_ownership_global_batch /=.
+          rewrite -H0 vlookup_insert.
+          destruct H1;split;eauto.
+          generalize dependent sps.
+          induction ps;simpl in *.
+          done.
+          intros.
+          destruct (decide (x=a)).
+          subst a.
+          rewrite lookup_insert.
+          rewrite /is_owned in H3.
+          destruct x0;eauto.
+          done.
+          rewrite lookup_insert_ne;eauto.
+          inv_map_in.
+          exists (x,Owned).
           split;eauto.
-          rewrite -H3.
-          do 8 f_equal.
+          apply elem_of_list_In .
+          apply elem_of_map_to_list.
+          apply map_filter_lookup_Some.
+          rewrite /get_vm_page_table /get_page_tables /update_ownership_batch
+                  /update_ownership_global_batch /=.
+          split;eauto.
+          rewrite -H0 vlookup_insert //=.
+          generalize dependent sps.
+          induction ps;simpl in *.
+          intros.
+          set_solver.
+          intros.
+          destruct (decide (x=a)).
+          subst a.
+          rewrite lookup_insert //.
+          rewrite lookup_insert_ne;eauto.
+          apply (IHps (list_to_set ps));eauto.
+          set_solver.
+      }
+      apply (@elem_of_list_to_map_1' VMID (gmap VMID) _ _ _ _ _ _ _ _ gmap_finmap).
+      + intros.
+        inv_map_in.
+        inversion H2.
+        do 3 f_equal.
+        clear H6 H3 H2.
+        subst x.
+        symmetry.
+        apply Hgoal.
+      + inv_map_in.
+        exists i.
+        split;[|apply in_list_of_vmids].
+        do 4 f_equal.
+        apply Hgoal.
+    - rewrite (lookup_insert_ne _ i i0 _);eauto.
+      set (l:= (map
+                  (λ v : VMID,
+                    (v, (GSet
+                           (list_to_set
+                              (map (λ p : PID * ownership, p.1)
+                                   (map_to_list
+                                      (filter (λ p : PID * ownership, is_owned p.2 = true) (get_vm_page_table σ v).1)))))))
+                  list_of_vmids)) in *.
+      destruct (list_to_map l !! i0) eqn:Heqn.
+      + apply (elem_of_list_to_map_2 l i0 g) in Heqn.
+        apply elem_of_list_In in Heqn.
+        apply in_map_iff in Heqn.
+        inversion Heqn;clear Heqn.
+        destruct H2 as [H3 HIn];inversion H3;subst;clear H3.
+        apply (@elem_of_list_to_map_1' VMID (gmap VMID) _ _ _ _ _ _ _ _ gmap_finmap).
+        *  intros.
+           inv_map_in.
+           inversion H.
+           do 5 f_equal.
+           rewrite /get_vm_page_table update_ownership_batch_preserve_other_page_tables //.
+        * inv_map_in.
+          exists i0.
+          split;eauto.
+          do 6 f_equal.
           rewrite /get_vm_page_table update_ownership_batch_preserve_other_page_tables //.
-          destruct x.
-          simpl in H2;inversion H3.
-          by subst.
-    Qed.
+      + apply (@not_elem_of_list_to_map_2 VMID (gmap VMID) _ _ _ _ _ _ _ _ gmap_finmap) in Heqn.
+        apply (@not_elem_of_list_to_map_1 VMID (gmap VMID) _ _ _ _ _ _ _ _ gmap_finmap).
+        intro P.
+        apply Heqn.
+        apply elem_of_list_In.
+        apply in_map_iff.
+        apply elem_of_list_In in P.
+        apply in_map_iff in P.
+        destruct P.
+        exists x.
+        destruct H2.
+        split;eauto.
+        apply in_map_iff.
+        apply in_map_iff in H3.
+        destruct H3.
+        exists x0.
+        destruct H3.
+        split;eauto.
+        rewrite -H3.
+        do 6 f_equal.
+        rewrite /get_vm_page_table update_ownership_batch_preserve_other_page_tables //.
+        destruct x.
+        simpl in H2;inversion H3.
+        by subst.
+  Qed.
 
   Lemma insert_transaction_preserve_current_vm σ h trans:
    get_current_vm (insert_transaction σ h trans) = get_current_vm σ.
